{
 "cells": [
  {
   "cell_type": "markdown",
   "metadata": {
    "id": "tx_w5JEYbNGy"
   },
   "source": [
    "\n",
    "\n",
    "$\\textbf{Assignment 1}$\n",
    "\n",
    "To prove that Euler's number, $( e )$, is irrational, we start by assuming the opposite, that is, $( e )$ can be expressed as a fraction $( \\frac{p}{q} )$, where $( p )$ and $( q )$are integers with no common factors other than 1, and $( q \\neq 0 )$.\n",
    "\n",
    "We recall the definition of $( e )$ as the sum of the infinite series:\n",
    "\n",
    "$[\n",
    "e = \\sum_{k=0}^\\infty \\frac{1}{k!}\n",
    "]$\n",
    "\n",
    "Let's denote the $( n )$th partial sum of this series as $( S_n ):$\n",
    "\n",
    "$[\n",
    "S_n = \\sum_{k=0}^n \\frac{1}{k!}\n",
    "]$\n",
    "\n",
    "Since we assumed $( e )$ is rational, $( S_n )$ must approach a rational limit as $( n)$ goes to infinity. However, since each term in the series $( \\frac{1}{k!} )$ is positive, $( S_n )$ is increasing.\n",
    "\n",
    "We know that for any $( k \\geq 1 )$, $( k! > k )$, which implies $( \\frac{1}{k!} < \\frac{1}{k} )$. This means that the series $( \\sum_{k=0}^\\infty \\frac{1}{k!} )$ converges.\n",
    "\n",
    "Now, if $( S_n )$ converges to a rational number, it must be bounded. However, this contradicts the divergence of the harmonic series, which is made of larger terms.\n",
    "\n",
    "Hence, assuming $( e )$ is rational leads to a contradiction. Therefore, we conclude that $( e )$ is not rational, i.e., $( e \\notin \\mathbb{Q} )$.\n",
    "\n",
    "\n",
    "<br><br>\n",
    "\n",
    "2. $\\textbf{Assignment 2}$\n",
    "\n",
    "We aim to prove Minkowski's Inequality for sums of positive real numbers $( (a_k, b_k) > 0 )$ and $( p > 1 )$:\n",
    "\n",
    "$\n",
    "\\begin{equation}\n",
    "\\left( \\sum_{k=1}^n |a_k + b_k|^p \\right)^\\frac{1}{p} \\leq \\left( \\sum_{k=1}^n |a_k|^p \\right)^\\frac{1}{p} + \\left( \\sum_{k=1}^n |b_k|^p \\right)^\\frac{1}{p}\n",
    "\\end{equation}\n",
    "$\n",
    "$\n",
    "\\\\ \\textbf{Step 1: Power-of-a-Power Rule}\n",
    "$\n",
    "We know that $( (n^p)^\\frac{1}{p} = n )$ for any base number $( n )$. Applying this to the sums of absolute values raised to the power of $( p )$, we can rewrite the inequality:\n",
    "\n",
    "$\n",
    "\\begin{equation}\n",
    "\\sum_{k=1}^n |a_k + b_k| \\leq \\sum_{k=1}^n |a_k| + \\sum_{k=1}^n |b_k|\n",
    "\\end{equation}\n",
    "$\n",
    "\n",
    "$\\\\ \\textbf{Step 2: Property of Summation}$\n",
    "\n",
    "The summation operation $( \\sum )$ distributes over addition. Therefore:\n",
    "\n",
    "$\n",
    "\\begin{equation}\n",
    "\\sum_{k=1}^n |a_k + b_k| \\leq \\sum_{k=1}^n |a_k| + \\sum_{k=1}^n |b_k|\n",
    "\\end{equation}\n",
    "$\n",
    "$\\\\ \\textbf{Step 3: Triangle Inequality}$\n",
    "\n",
    "For clarity, let's remove the summation notation:\n",
    "\n",
    "$[ |a_k + b_k| \\leq |a_k| + |b_k| ]$\n",
    "\n",
    "Since $( (a_k, b_k) > 0 )$, both $( a_k )$ and $( b_k )$ are positive real numbers. This guarantees that $( (a_k + b_k) )$ is also positive, and the absolute value operation doesn't change the sign. Therefore, $( |a_k + b_k| = a_k + b_k )$. Similarly, $( |a_k| = a_k )$ and $( |b_k| = b_k )$.\n",
    "\n",
    "Substituting these equalities, we get:\n",
    "\n",
    "$[ a_k + b_k \\leq a_k + b_k ]$\n",
    "\n",
    "This is trivially true, demonstrating that the inequality holds for any positive real numbers $( a_k )$ and $( b_k )$.\n",
    "\n",
    "$\\\\ \\textbf{Conclusion}$\n",
    "\n",
    "By utilizing the power-of-a-power rule, the property of summation, and the triangle inequality, we have proven Minkowski's Inequality for sums of positive real numbers with $( p > 1 )$.\n",
    "\n",
    "<br><br>\n",
    "\n",
    "\n",
    "\n",
    "$\\textbf{Assignment 3}$\n",
    "\n",
    "$\\textbf{Step 1: Definition of an absolute value}$\n",
    "\n",
    "$\\textbf{Definition}\n",
    "\\begin{equation}\n",
    "{|x| = }\n",
    "\\begin{cases}\n",
    "x, & \\text{if } x \\geq 0 \\\\\n",
    "-x, & \\text{if } x < 0\n",
    "\\end{cases}\n",
    "\\end{equation}$\n",
    "\n",
    "Thus, we must solve for 4 cases:\n",
    "$\n",
    "\\begin{align}\n",
    "\\text{Case 1: } & \\text{if } x \\geq 0, y \\geq 0 \\\\\n",
    "\\text{Case 2: } & \\text{if } x < 0, y < 0 \\\\\n",
    "\\text{Case 3: } & \\text{if } x \\geq 0, y < 0 \\\\\n",
    "\\text{Case 4: } & \\text{if } x < 0, y \\geq 0\n",
    "\\end{align}\n",
    "$\n",
    "$\\textbf{Case 1:} ( x \\geq 0, y \\geq 0 )$\n",
    "$\n",
    "Let $( |x + y| = x + y )$, $( |x| = x )$, and $( |y| = y )$.\n",
    "Substitution:\n",
    "\\begin{equation}\n",
    "|x + y| = x + y = |x| + |y|\n",
    "\\end{equation}\n",
    "$\n",
    "\n",
    "$\\textbf{Case 2:} ( x < 0, y < 0 )$\n",
    "\n",
    "Let $( |x + y| = -(x + y) )$, $( |x| = -x )$, and $( |y| = -y )$.\n",
    "$\n",
    "Substitution:\n",
    "\\begin{equation}\n",
    "|x + y| = -(x + y) = -x + (-y) = |x| + |y|\n",
    "\\end{equation}\n",
    "$\n",
    "$\\textbf{Case 3:} ( x \\geq 0, y < 0 )$\n",
    "\n",
    "Let $( |x| = x )$ and $( |y| = -y )$.\n",
    "Substitution:\n",
    "$\n",
    "\\begin{equation}\n",
    "|x + y| \\leq x - y\n",
    "\\end{equation}\n",
    "$\n",
    "Since $( x )$ is non-negative and $( y )$ is negative, $( x - y )$ could be either positive or negative. So, let's consider both possibilities:\n",
    "\n",
    "For $( x + y \\geq 0 )$:\n",
    "$\\begin{align}\n",
    "x + y & \\leq x - y \\\\\n",
    "y & \\leq -y\n",
    "\\end{align}\n",
    "$\n",
    "\n",
    "For $( x + y < 0 )$:\n",
    "$\\begin{align}\n",
    "-(x + y) & \\leq x - y \\\\\n",
    "-x - y & \\leq x - y \\\\\n",
    "-x & \\leq x\n",
    "\\end{align}$\n",
    "\n",
    "$\\textbf{Case 4:} ( x < 0, y \\geq 0 )$\n",
    "\n",
    "Let $( |x| = -x )$ and $( |y| = y )$.\n",
    "Substitution:\n",
    "$\n",
    "\\begin{equation}\n",
    "|x + y| \\leq -x + y\n",
    "\\end{equation}\n",
    "Solve for sub-cases of ( |x + y| ):\n",
    "\\begin{align}\n",
    "x + y, & x + y \\geq 0 \\\\\n",
    "-(x + y), & x + y < 0 \\\\\n",
    "\\end{align}\n",
    "$\n",
    "For $( x + y \\geq 0 )$:\n",
    "$\n",
    "\\begin{align}\n",
    "x + y & \\leq -x + y \\\\\n",
    "x & \\leq -x\n",
    "\\end{align}\n",
    "$\n",
    "\n",
    "For $( x + y < 0 )$:\n",
    "$\n",
    "\\begin{align}\n",
    "-(x + y) & \\leq -x + y \\\\\n",
    "-x - y & \\leq -x + y \\\\\n",
    "-y & \\leq y\n",
    "\\end{align}\n",
    "$\n",
    "\n",
    "$\\textbf{In Conclusion}$, in all cases, $( |x+y| \\leq |x| + |y| \\in \\mathbb{R} )$.\n",
    "\n",
    "\n",
    "\n",
    "\n",
    "<br> <br>\n",
    "\n",
    "$\\textbf{Assignment 4$\n",
    "\n",
    "4. Prove Sedrakayan's Lemma $\\forall u_i, v_i \\in \\mathbb{R}^+$:\n",
    "\\begin{gather}\n",
    "\\frac{(\\Sigma_{i=1}^n u_i)^2}{\\Sigma_{i=1}^n v_i}\n",
    "\\leq\n",
    "\\Sigma_{i=1}^n \\frac{(u_i)^2}{v_i}\n",
    "\\end{gather}\n",
    "\n",
    "We will prove Sedrakayan's Lemma for non-negative real numbers $(u_i, v_i) \\in \\mathbb{R}^+$:\n",
    "\n",
    "$$\\frac{\\left( \\sum\\limits_{i=1}^n u_i \\right)^2}{\\sum\\limits_{i=1}^n v_i} \\leq \\sum\\limits_{i=1}^n \\frac{u_i^2}{v_i}$$\n",
    "\n",
    "$\\textbf{Step 1}$\n",
    "the Cauchy-Schwarz Inequality\n",
    "\n",
    "$$\\left( \\frac{\\sum\\limits_{i=1}^n u_i}{\\sum\\limits_{i=1}^n v_i} \\right)^2 \\leq \\frac{\\sum\\limits_{i=1}^n u_i^2}{v_i}$$\n",
    "\n",
    "$\\textbf{Step 2}$\n",
    "\n",
    "The Cauchy-Schwarz Inequality states that for any real numbers $(a_i)$ and $(b_i)$:\n",
    "\n",
    "$$\\left( \\sum\\limits_{i=1}^n a_i b_i \\right)^2 \\leq \\left( \\sum\\limits_{i=1}^n a_i^2 \\right) \\left( \\sum\\limits_{i=1}^n b_i^2 \\right)$$\n",
    "\n",
    "\n",
    "$\\textbf{Step 3}$\n",
    "\n",
    "Let's define:\n",
    "\n",
    "* $a_i = \\sqrt{u_i}$\n",
    "* $b_i = \\frac{1}{\\sqrt{v_i}}$\n",
    "\n",
    "$$\\left( \\sum\\limits_{i=1}^n \\sqrt{u_i} \\cdot \\frac{1}{\\sqrt{v_i}} \\right)^2 \\leq \\left( \\sum\\limits_{i=1}^n u_i \\right) \\left( \\sum\\limits_{i=1}^n \\frac{1}{v_i} \\right)$$\n",
    "\n",
    "$\\textbf{Step 4}$\n",
    "\n",
    "* **Left-hand side:**\n",
    "\n",
    "$$\\left( \\sum\\limits_{i=1}^n \\sqrt{u_i} \\cdot \\frac{1}{\\sqrt{v_i}} \\right)^2 = \\left( \\frac{\\sum\\limits_{i=1}^n u_i}{\\sum\\limits_{i=1}^n v_i} \\right)^2$$\n",
    "\n",
    "\n",
    "* **Right-hand side:**\n",
    "\n",
    "$$\\left( \\sum\\limits_{i=1}^n u_i \\right) \\left( \\sum\\limits_{i=1}^n \\frac{1}{v_i} \\right) = \\frac{\\sum\\limits_{i=1}^n u_i^2}{v_i}$$\n",
    "\n",
    "\n",
    "$\\textbf{Step 5}$\n",
    "\n",
    "Since the reformulated inequality on the left-hand side is less than or equal to the right-hand side, as derived from the Cauchy-Schwarz Inequality, we have successfully demonstrated the validity of Sedrakayan's Lemma for all non-negative real numbers.$(u_i, v_i) \\in \\mathbb{R}^+$.\n",
    "\n",
    "\n"
   ]
  },
  {
   "cell_type": "code",
   "execution_count": null,
   "metadata": {},
   "outputs": [],
   "source": []
  },
  {
   "cell_type": "code",
   "execution_count": null,
   "metadata": {},
   "outputs": [],
   "source": []
  }
 ],
 "metadata": {
  "colab": {
   "provenance": []
  },
  "kernelspec": {
   "display_name": "Python 3 (ipykernel)",
   "language": "python",
   "name": "python3"
  },
  "language_info": {
   "codemirror_mode": {
    "name": "ipython",
    "version": 3
   },
   "file_extension": ".py",
   "mimetype": "text/x-python",
   "name": "python",
   "nbconvert_exporter": "python",
   "pygments_lexer": "ipython3",
   "version": "3.11.4"
  }
 },
 "nbformat": 4,
 "nbformat_minor": 4
}
